Structure the proof of reordering

src/opt/Reorder.v
@@ -78,12 +78,12 @@ Inductive reordered_thread: forall (text1 text2:Thread.syntax), Prop :=
       (Thread.mk_syntax lang s2)
 .
 
-Inductive reordered_program i: forall (prog1 prog2:Configuration.syntax), Prop :=
+Inductive reordered_program tid: forall (prog1 prog2:Configuration.syntax), Prop :=
 | reordered_program_intro
     prog1 th1 th2
-    (TH1: IdentMap.find i prog1 = Some th1)
+    (TH1: IdentMap.find tid prog1 = Some th1)
     (REORDER: reordered_thread th1 th2):
-    reordered_program i prog1 (IdentMap.add i th2 prog1)
+    reordered_program tid prog1 (IdentMap.add tid th2 prog1)
 .
 
 Inductive consumed_stmts (i2:Instr.t): forall (c1 c2:list Stmt.t), Prop :=
@@ -114,11 +114,11 @@ Proof.
   inv SIM. eexists _, _, _. splits; eauto.
 Qed.
 
-Inductive sim_consumed_thread (e:option RWEvent.t): forall (th1 th2:Thread.t), Prop :=
+Inductive sim_consumed_thread (e:option MemEvent.t): forall (th1 th2:Thread.t), Prop :=
 | sim_consumed_thread_intro
-    rs1 rs2 s1 s2 i
-    (CONSUMED: consumed_stmts i s1 s2)
-    (EVAL: RegFile.eval_instr rs1 i (option_map (ThreadEvent.mem <*> ThreadEvent.rw) e) rs2):
+    rs1 rs2 s1 s2 tid
+    (CONSUMED: consumed_stmts tid s1 s2)
+    (EVAL: RegFile.eval_instr rs1 tid (option_map ThreadEvent.mem e) rs2):
     sim_consumed_thread
       e
       (Thread.mk lang (State.mk rs1 s1))
@@ -128,225 +128,104 @@ Inductive sim_consumed_thread (e:option RWEvent.t): forall (th1 th2:Thread.t), P
 (* TODO: refactoring *)
 Lemma sim_consumed_thread_inv
       e th1 th2 (SIM: sim_consumed_thread e th1 th2):
-  exists rs1 rs2 s1 s2 i,
+  exists rs1 rs2 s1 s2 tid,
     th1 = Thread.mk lang (State.mk rs1 s1) /\
     th2 = Thread.mk lang (State.mk rs2 s2) /\
-    consumed_stmts i s1 s2 /\
-    RegFile.eval_instr rs1 i (option_map (ThreadEvent.mem <*> ThreadEvent.rw) e) rs2.
+    consumed_stmts tid s1 s2 /\
+    RegFile.eval_instr rs1 tid (option_map ThreadEvent.mem e) rs2.
 Proof.
   inv SIM. eexists _, _, _, _, _. splits; eauto.
 Qed.
 
-Definition sim_message (msg1 msg2:Message.t): bool :=
-  match msg1, msg2 with
-  | Message.rw (RWEvent.read l1 c1 o1) t1,
-    Message.rw (RWEvent.write l2 c2 o2) t2 =>
-    (negb (Loc.eqb l1 l2)) &&
-    (negb (Ordering.ord Ordering.acquire o1)) &&
-    (negb (Ordering.ord Ordering.release o2))
-  | _, _ =>
-    false
-  end.
-
-Inductive sim_buffer: forall (b1 b2:Buffer.t), Prop :=
-| sim_buffer_nil:
-    sim_buffer nil nil
-| sim_buffer_cons
-    msg b1 b2
-    (BUFFER: sim_buffer b1 b2):
-    sim_buffer (b1 ++ [msg]) (b2 ++ [msg])
-| sim_buffer_reorder
-    msg1 msg2 b1 b2
-    (MSG: sim_message msg1 msg2)
-    (BUFFER: sim_buffer b1 b2):
-    sim_buffer (b1 ++ [msg1; msg2]) (b2 ++ [msg2; msg1])
+(* TODO *)
+Inductive sim_thread
+          (commit1 commit2:Commit.t)
+          (th1 th2:Thread.t)
+          (messages1 messages2:Messages.t): Prop :=
+| sim_thread_reordered
+    (COMMIT: commit1 = commit2)
+    (TH: sim_reordered_thread th1 th2)
+    (MESSAGES: messages1 = messages2)
+| sim_thread_consumed
+    (TODO: False)
 .
 
-Inductive sim_consumed_buffer: forall (e:option (RWEvent.t * nat)) (b1 b2:Buffer.t), Prop :=
-| sim_consumed_buffer_None
-    b1 b2
-    (BUFFER: sim_buffer b1 b2):
-    sim_consumed_buffer None b1 b2
-| sim_consumed_buffer_Some
-    e ts b1 b2
-    (BUFFER: sim_buffer b1 b2):
-    sim_consumed_buffer (Some (e, ts)) b1 (b2 ++ [Message.rw e ts])
-.
-
-Inductive sim_inceptions i: forall (e:option (RWEvent.t * nat)) (inceptions1 inceptions2:InceptionSet.t), Prop :=
-| sim_inceptions_None inceptions:
-    sim_inceptions i None inceptions inceptions
-| sim_inceptions_Some
-    e ts inceptions2:
-    sim_inceptions
-      i (Some (e, ts))
-      (InceptionSet.add (Inception.mk e ts (IdentSet.singleton i)) inceptions2)
-      inceptions2
-.
-
-Inductive sim_context i:
-  forall (c1 c2:Clock.t)
-    (th1 th2:Thread.t)
-    (b1 b2:Buffer.t)
-    (inceptions1 inceptions2:InceptionSet.t), Prop :=
-| sim_context_reordered
-    c1 c2 th1 th2 b1 b2 inceptions1 inceptions2
-    (CLOCK: c1 = c2)
-    (THREAD: sim_reordered_thread th1 th2)
-    (BUFFER: sim_buffer b1 b2)
-    (INCEPTIONS: inceptions1 = inceptions2):
-    sim_context i c1 c2 th1 th2 b1 b2 inceptions1 inceptions2
-| sim_context_consumed
-    c1 c2 th1 th2 b1 b2 inceptions1 inceptions2
-    e
-    (CLOCK: Clock.le c1 c2)
-    (THREAD2: sim_consumed_thread (option_map fst e) th1 th2)
-    (BUFFER2: sim_consumed_buffer e b1 b2)
-    (INCEPTIONS: sim_inceptions i e inceptions1 inceptions2):
-    sim_context i c1 c2 th1 th2 b1 b2 inceptions1 inceptions2
-.
-
-Inductive sim_configuration i: forall (conf1 conf2:Configuration.t), Prop :=
+Inductive sim_configuration tid (conf1 conf2:Configuration.t): Prop :=
 | sim_configuration_intro
-    c1 c2 th1 th2 b1 b2 inceptions1 inceptions2
-    p1 p2 bs1 bs2
-    (PROGRAM1: IdentMap.find i p1 = Some th1)
-    (BUFFER1: IdentFun.find i bs1 = b1)
-    (PROGRAM2: p2 = IdentMap.add i th2 p1)
-    (BUFFER2: bs2 = IdentFun.add i b2 bs1)
-    (CONTEXT: sim_context i c1 c2 th1 th2 b1 b2 inceptions1 inceptions2):
-    sim_configuration
-      i
-      (Configuration.mk c1 p1 (Memory.mk bs1 inceptions1))
-      (Configuration.mk c2 p2 (Memory.mk bs2 inceptions2))
+    commit1 commit2 th1 th2
+    (CONTEXT: forall i (TID: i <> tid),
+        IdentMap.find i conf1.(Configuration.threads) = IdentMap.find i conf2.(Configuration.threads))
+    (TH1: IdentMap.find tid conf1.(Configuration.threads) = Some (commit1, th1))
+    (TH2: IdentMap.find tid conf2.(Configuration.threads) = Some (commit2, th2))
+    (TH: sim_thread
+           commit1 commit2
+           th1 th2
+           conf1.(Configuration.messages) conf2.(Configuration.messages))
 .
 
 Lemma sim_init
-      i prog_src prog_tgt
-      (REORDER: reordered_program i prog_src prog_tgt):
-  Simulation.INIT prog_src prog_tgt (sim_configuration i).
+      tid prog_src prog_tgt
+      (REORDER: reordered_program tid prog_src prog_tgt):
+  Simulation.INIT prog_src prog_tgt (sim_configuration tid).
 Proof.
-  inv REORDER. repeat econs.
-  - unfold Program.init.
-    rewrite IdentMap.Facts.map_o, TH1.
-    simpl. eauto.
-  - apply IdentMap.map_add.
-  - rewrite IdentFun.add_init. auto.
-  - inv REORDER0. econs. eauto.
+  inv REORDER. unfold Simulation.INIT, Configuration.init.
+  econs; simpl; eauto.
+  - i. rewrite ? IdentMap.Facts.map_o.
+    rewrite IdentMap.Facts.add_neq_o; auto.
+  - rewrite IdentMap.Facts.map_o.
+    rewrite TH1. simpl. eauto.
+  - rewrite IdentMap.Facts.map_o.
+    rewrite IdentMap.Facts.add_eq_o; auto. simpl. eauto.
+  - econs 1; auto. inv REORDER0. econs; eauto.
 Qed.
 
-Lemma sim_feasible i: Simulation.FEASIBLE (sim_configuration i).
+Lemma sim_feasible tid: Simulation.FEASIBLE (sim_configuration tid).
 Proof.
-  ii. inversion SIM. subst. simpl in *.
-  inv CONTEXT.
-  { repeat econs. auto. }
-  inv INCEPTIONS.
-  { repeat econs. auto. }
-  simpl in *. inv THREAD2. inv BUFFER2. inv CONSUMED. simpl in *.
-  econs; [econs 2; [|econs 2; [|econs 1]]|].
-  - admit. (* we can execute i1 *)
-  - admit. (* we can execute i0 *)
-  - admit. (* the execution of i0 removes the only inception *)
+  ii. inv SIM. inv TH.
+  - econs.
+    + apply Configuration.steps_nil.
+    + rewrite MESSAGES. auto.
+  - admit. (* consumed *)
 Admitted.
 
-Lemma sim_Memory_message c1 c2 m1 m2 i e msg
-      (CLOCK: Clock.le c1 c2)
-      (MESSAGE: Memory.message c2 m2 i e msg):
-  Memory.message c1 m1 i e msg.
-Proof.
-  inv MESSAGE.
-  - econs.
-    admit.
-  - econs.
-    admit.
-  - econs.
-    admit.
-    admit.
-  - econs.
-Admitted.
-
-Lemma sim_base i: Simulation.BASE_STEP (sim_configuration i).
+Lemma sim_base tid: Simulation.BASE_STEP (sim_configuration tid).
 Proof.
   ii. inv SIM. inv STEP.
-  destruct (Ident.eq_dec i i0).
-  - subst i0. inv PROGRAM.
-    rewrite IdentMap.Facts.add_eq_o in *; auto.
-    inv THREAD. inv STEP. inv CONTEXT.
-    + apply sim_reordered_thread_inv in THREAD. des. subst.
-      inv THREAD0. apply inj_pair2 in H1. subst.
-      admit. (* program step, sim *)
-    + apply sim_consumed_thread_inv in THREAD2. des. subst.
-      inv THREAD0. apply inj_pair2 in H1. subst.
-      inv THREAD1.
-      admit. (* reordered instr should emit mem events: REORDER & STEP0 *)
-  - inv PROGRAM. rewrite IdentMap.Facts.add_neq_o in *; auto.
-    inv MEMORY.
-    + eexists _, _. splits.
-      * econs 1.
-      * econs 1. repeat (econs; eauto).
-      * econs; eauto.
-        { rewrite IdentMap.Facts.add_neq_o; auto. }
-        { apply IdentMap.add_add. auto. }
-    + eexists _, _. splits; eauto.
-      * econs 1.
-      * econs 1. econs.
-        { repeat (econs; eauto). }
-        econs.
-        { admit. (* Memory.message *) }
-        { unfold Memory.add_message. simpl in *. eauto. }
-      * econs; eauto.
-        { rewrite IdentMap.Facts.add_neq_o; eauto. }
-        { apply IdentMap.add_add. auto. }
-        admit. (* sim_context *)
+  - admit. (* tau *)
+  - admit. (* read *)
+  - admit. (* write *)
+  - admit. (* update *)
+  - admit. (* fence *)
+  - admit. (* declare *)
+  - admit. (* commit *)
 Admitted.
 
-Lemma sim_inception i: Simulation.INCEPTION_STEP (sim_configuration i).
+Lemma sim_external tid: Simulation.EXTERNAL_STEP (sim_configuration tid).
 Proof.
 Admitted.
 
-Lemma sim_external i: Simulation.EXTERNAL_STEP (sim_configuration i).
-Proof.
-  ii. inv SIM. inv STEP.
-  - eexists _, _. splits.
-    + econs 1.
-    + econs 1. inv CONTEXT; eauto.
-      admit. (* Clock.le transitive *)
-    + econs; eauto.
-      inv CONTEXT; [econs 1|econs 2]; eauto.
-      admit. (* Clock.le reflexive *)
-  - inv PROGRAM. inv STEP. simpl in *.
-    rewrite IdentMap.Facts.add_o in *. destruct (IdentMap.Facts.eq_dec i i0).
-    + subst. 
-      admit. (* the reordered thread syscalled *)
-    + eexists _, _. splits.
-      * econs 1.
-      * econs 2; simpl in *.
-        { econs; eauto. econs. eauto. }
-        { admit. (* inceptions *) }
-      * econs; eauto.
-        { rewrite IdentMap.Facts.add_neq_o; auto. }
-        { apply IdentMap.add_add. auto. }
-Admitted.
-
-Lemma sim_terminal i: Simulation.TERMINAL (sim_configuration i).
+Lemma sim_terminal tid: Simulation.TERMINAL (sim_configuration tid).
 Proof.
   ii. eexists. split.
   { apply Configuration.steps_nil. }
-  econs. econs. i.
-  inv TERM. inv PROGRAM. specialize (TERMINAL i0).
-  inv SIM. simpl in *.
-  rewrite IdentMap.Facts.add_o in *.
-  destruct (IdentMap.Facts.eq_dec i i0); auto.
-  subst. exploit TERMINAL; eauto. intro X.
-  rewrite PROGRAM1 in THREAD. inv THREAD.
-  inv CONTEXT.
-  - inv THREAD. inv X. simpl in *. subst. inv REORDER. auto.
-  - inv THREAD2. inv X. simpl in *. subst. inv CONSUMED.
-Qed.
+  econs. i. inv TERM. specialize (TERMINAL tid0).
+  destruct (Ident.eq_dec tid0 tid); subst.
+  - inv SIM. inv TH.
+    + rewrite FIND in TH1. inv TH1.
+      exploit TERMINAL; eauto.
+      unfold Thread.is_terminal. inv TH0. simpl.
+      unfold State.is_terminal. simpl.
+      inv REORDER; congruence.
+    + rewrite FIND in TH1. inv TH1.
+      exploit TERMINAL; eauto.
+      admit. (* consumed *)
+  - inv SIM. exploit CONTEXT; eauto. intro FIND0.
+    eapply TERMINAL. rewrite <- FIND0. eauto.
+Admitted.
 
 Definition sim
-           i prog_src prog_tgt
-           (REORDER: reordered_program i prog_src prog_tgt):
+           tid prog_src prog_tgt
+           (REORDER: reordered_program tid prog_src prog_tgt):
   Simulation.t prog_src prog_tgt :=
   Simulation.mk
     _ _
@@ -354,6 +233,5 @@ Definition sim
     (Simulation.step_lemma
        (@sim_feasible _)
        (@sim_base _)
-       (@sim_inception _)
        (@sim_external _))
     (@sim_terminal _).
